Cil2Csyntax: added goto and labels; added assignment between structs Kildall: simplified the interface Constprop, CSE, Allocation, Linearize: updated for the new Kildall RTL, LTL: removed the well-formedness condition on the CFG,   it is no longer necessary with the new Kildall and it is problematic   for validated optimizations. Maps: more efficient implementation of PTree.fold.
git-svn-id: https://yquem.inria.fr/compcert/svn/compcert/trunk@1124 fca1b0fc-160b-0410-b1d3-a4f43f01ea2e

backend/Linearizeaux.ml
@@ -50,6 +50,7 @@ module IntSet = Set.Make(struct type t = int let compare = compare end)
 (* Determine join points: reachable nodes that have > 1 predecessor *)
 
 let join_points f =
+  let succs = LTL.successors f in
   let reached = ref IntSet.empty in
   let reached_twice = ref IntSet.empty in
   let rec traverse pc =
@@ -59,7 +60,7 @@ let join_points f =
         reached_twice := IntSet.add npc !reached_twice
     end else begin
       reached := IntSet.add npc !reached;
-      List.iter traverse (LTL.successors f pc)
+      List.iter traverse (Kildall.successors_list succs pc)
     end
   in traverse f.fn_entrypoint; !reached_twice
 
